theories/lifting.v
@@ -72,6 +72,18 @@ Notation "'WPexp' e {{ v , Q } }" := (wp_exp e (λ v, Q))
   (at level 20, e, Q at level 200,
    format "'[' 'WPexp'  e  '/' '[   ' {{  v ,  Q  } } ']' ']'") : bi_scope.
 
+Definition wp_a_exp_def `{!islaG Σ} `{!threadG} (e : a_exp) (Φ : base_val → iProp Σ) : iProp Σ :=
+  (∀ regs, thread_ctx regs -∗ ∃ v, ⌜eval_a_exp regs e = Some v⌝ ∗ thread_ctx regs ∗ Φ v).
+Definition wp_a_exp_aux `{!islaG Σ} `{!threadG} : seal (@wp_a_exp_def Σ _ _). by eexists. Qed.
+Definition wp_a_exp `{!islaG Σ} `{!threadG} : a_exp → (base_val → iProp Σ ) → iProp Σ := (wp_a_exp_aux).(unseal).
+Definition wp_a_exp_eq `{!islaG Σ} `{!threadG} : wp_a_exp = @wp_a_exp_def Σ _ _ := (wp_a_exp_aux).(seal_eq).
+
+Notation "'WPaexp' e {{ Φ } }" := (wp_a_exp e%E Φ)
+  (at level 20, e, Φ at level 200, only parsing) : bi_scope.
+Notation "'WPaexp' e {{ v , Q } }" := (wp_a_exp e (λ v, Q))
+  (at level 20, e, Q at level 200,
+   format "'[' 'WPaexp'  e  '/' '[   ' {{  v ,  Q  } } ']' ']'") : bi_scope.
+
 Ltac inv_seq_step :=
   simplify_eq/=;
   lazymatch goal with
@@ -79,7 +91,7 @@ Ltac inv_seq_step :=
   end;
   simplify_eq/=;
   lazymatch goal with
-  | H : trace_step _ _ _ |- _ => inversion H; clear H
+  | H : trace_step _ _ _ _ |- _ => inversion H; clear H
   end;
   simplify_eq/=;
   destruct_and?;
@@ -95,6 +107,9 @@ Section lifting.
   Lemma wp_exp_unfold e Φ:
     WPexp e {{ Φ }} ⊣⊢ wp_exp_def e Φ.
   Proof. by rewrite wp_exp_eq. Qed.
+  Lemma wp_a_exp_unfold e Φ:
+    WPaexp e {{ Φ }} ⊣⊢ wp_a_exp_def e Φ.
+  Proof. by rewrite wp_a_exp_eq. Qed.
 
   Global Instance elim_modal_bupd_wp_asm p P es :
     ElimModal True p false (|==> P) P (WPasm es) (WPasm es).
@@ -322,6 +337,60 @@ Section lifting.
     (⌜v = v'⌝ -∗ r ↦ᵣ{q} v' -∗ WPasm es) -∗
     WPasm (ReadReg r [] v ann :: es).
   Proof. by apply: wp_read_reg_acc. Qed.
+
+  Lemma wp_assume_reg_acc r v v' ann es q al:
+    read_accessor al v' = Some v →
+    r ↦ᵣ{q} v' -∗
+    (r ↦ᵣ{q} v' -∗ WPasm es) -∗
+    WPasm (AssumeReg r al v ann :: es).
+  Proof.
+    iIntros (?) "Hr Hcont". setoid_rewrite wp_asm_unfold.
+    iIntros ([???]) "/= -> -> Hθ".
+    iApply wp_lift_step; [done|].
+    iIntros (σ1 ??? ?) "(?&Hictx&?)".
+    iApply fupd_mask_intro; first set_solver. iIntros "HE".
+    iDestruct (reg_mapsto_lookup with "Hθ Hr") as %Hr.
+    iSplit. {
+      iPureIntro. eexists _, _, _, _; simpl. econstructor; [done |by econstructor|]; simpl.
+      eexists _. split_and! => //.
+    }
+    iIntros "!>" (????). iMod "HE" as "_". iModIntro.
+    inv_seq_step. revert select (∃ x, _) => -[?[?[?[?[??]]]]]; simplify_eq/=.
+    unfold register_name in *. simplify_eq/=.
+    iFrame; iSplitL; [|done].
+    iApply ("Hcont" with "Hr"); [done|done|].
+    iFrame.
+  Qed.
+
+  Lemma wp_assume_reg_struct r v ann es q f:
+    r # f ↦ᵣ{q} v -∗
+    (r # f ↦ᵣ{q} v -∗ WPasm es) -∗
+    WPasm (AssumeReg r [Field f] v ann :: es).
+  Proof.
+    iIntros "Hr Hcont". setoid_rewrite wp_asm_unfold.
+    iIntros ([???]) "/= -> -> Hθ".
+    iApply wp_lift_step; [done|].
+    iIntros (σ1 ??? ?) "(?&Hictx&?)".
+    iApply fupd_mask_intro; first set_solver. iIntros "HE".
+    iDestruct (struct_reg_mapsto_lookup with "Hθ Hr") as %(?&?&?&?&?).
+    iSplit. {
+      iPureIntro. eexists _, _, _, _; simpl. econstructor; [done |by econstructor|]; simpl.
+      eexists _. split_and! => //=.
+      rewrite /read_accessor/=. by simplify_option_eq.
+    }
+    iIntros "!>" (????). iMod "HE" as "_". iModIntro.
+    inv_seq_step. revert select (∃ x, _) => -[?[?[?[?[??]]]]]; simplify_eq/=.
+    unfold register_name, read_accessor in *. simplify_option_eq.
+    iFrame; iSplitL; [|done].
+    iApply ("Hcont" with "Hr"); [done|done|].
+    iFrame.
+  Qed.
+
+  Lemma wp_assume_reg r v ann es q:
+    r ↦ᵣ{q} v -∗
+    (r ↦ᵣ{q} v -∗ WPasm es) -∗
+    WPasm (AssumeReg r [] v ann :: es).
+  Proof. by apply: wp_assume_reg_acc. Qed.
 
   Lemma wp_write_reg_acc r v v' v'' vnew ann es al:
     read_accessor al v = Some vnew →
@@ -620,10 +689,30 @@ Section lifting.
     iApply "Hcont"; [done|done|done|iFrame].
   Qed.
 
+  Lemma wp_assume es ann e:
+    WPaexp e {{ v, ⌜v = Val_Bool true⌝ ∗ WPasm es }} -∗
+    WPasm (Assume e ann :: es).
+  Proof.
+    rewrite wp_a_exp_unfold wp_asm_eq.
+    iIntros "Hexp" ([???]) "/= -> -> Hθ".
+    iDestruct ("Hexp" with "Hθ") as (v ?) "(Hθ&%&Hcont)"; subst.
+    iApply wp_lift_step; [done|].
+    iIntros (σ1 ??? ?) "Hctx".
+    iApply fupd_mask_intro; first set_solver. iIntros "HE".
+    iSplit. {
+      iPureIntro.
+      eexists _, _, _, _; econstructor; [done | by econstructor|done].
+    }
+    iIntros "!>" (????). iMod "HE" as "_". iModIntro.
+    inv_seq_step.
+    iFrame; iSplit; [|done].
+    iApply "Hcont"; [done|done|iFrame].
+  Qed.
+
 End lifting.
 
 Section exp_lifting.
-  Context `{!islaG Σ}.
+  Context `{!islaG Σ} `{!threadG}.
 
   Lemma wpe_wand e Φ1 Φ2:
     WPexp e {{ Φ1 }} -∗
@@ -634,10 +723,54 @@ Section exp_lifting.
     iExists _. iSplit; [done|]. by iApply "Hv".
   Qed.
 
+  Lemma wpae_wand e Φ1 Φ2:
+    WPaexp e {{ Φ1 }} -∗
+    (∀ v, Φ1 v -∗ Φ2 v) -∗
+    WPaexp e {{ Φ2 }}.
+  Proof.
+    rewrite !wp_a_exp_unfold.
+    iIntros "Hexp HΦ" (regs) "Hregs".
+    iDestruct ("Hexp" with "Hregs") as (??) "[??]".
+    iExists _. iSplit; [done|]. iFrame. by iApply "HΦ".
+  Qed.
+
   Lemma wpe_val v Φ ann:
     Φ v -∗
     WPexp (Val v ann) {{ Φ }}.
   Proof. rewrite wp_exp_unfold. iIntros "?". iExists _. by iFrame. Qed.
+
+  Lemma wpae_var_reg r q v Φ ann :
+    r ↦ᵣ{q} RegVal_Base v -∗
+    (r ↦ᵣ{q} RegVal_Base v -∗ Φ v) -∗
+    WPaexp (AExp_Val (AVal_Var r []) ann) {{ Φ }}.
+  Proof.
+    rewrite wp_a_exp_unfold. iIntros "Hr HΦ" (?) "Hregs" => /=.
+    iDestruct (reg_mapsto_lookup with "Hregs Hr") as %->.
+    iExists _ => /=. iSplit; [done|]. iFrame. by iApply "HΦ".
+  Qed.
+  Lemma wpae_var_struct r f q v Φ ann :
+    r # f ↦ᵣ{q} RegVal_Base v -∗
+    (r # f ↦ᵣ{q} RegVal_Base v -∗ Φ v) -∗
+    WPaexp (AExp_Val (AVal_Var r [Field f]) ann) {{ Φ }}.
+  Proof.
+    rewrite wp_a_exp_unfold. iIntros "Hr HΦ" (?) "Hregs" => /=.
+    iDestruct (struct_reg_mapsto_lookup with "Hregs Hr") as %[?[?[->[??]]]].
+    rewrite /read_accessor/=. simplify_option_eq.
+    iExists _ => /=. iSplit; [done|]. iFrame. by iApply "HΦ".
+  Qed.
+
+  Lemma wpae_bits b Φ ann:
+    Φ (Val_Bits b) -∗
+    WPaexp (AExp_Val (AVal_Bits b) ann) {{ Φ }}.
+  Proof. rewrite wp_a_exp_unfold. iIntros "?" (?) "?". iExists _. by iFrame. Qed.
+  Lemma wpae_bool b Φ ann:
+    Φ (Val_Bool b) -∗
+    WPaexp (AExp_Val (AVal_Bool b) ann) {{ Φ }}.
+  Proof. rewrite wp_a_exp_unfold. iIntros "?" (?) "?". iExists _. by iFrame. Qed.
+  Lemma wpae_enum b Φ ann:
+    Φ (Val_Enum b) -∗
+    WPaexp (AExp_Val (AVal_Enum b) ann) {{ Φ }}.
+  Proof. rewrite wp_a_exp_unfold. iIntros "?" (?) "?". iExists _. by iFrame. Qed.
 
   Lemma wpe_manyop op es Φ ann:
     foldr (λ e Ψ, λ vs, WPexp e {{ v, Ψ (vs ++ [v]) }}) (λ vs, ∃ v, ⌜eval_manyop op vs = Some v⌝ ∗ Φ v) es [] -∗
@@ -661,12 +794,44 @@ Section exp_lifting.
       constructor; [done|]. constructor.
   Qed.
 
+  Lemma wpae_manyop op es Φ ann:
+    foldr (λ e Ψ, λ vs, WPaexp e {{ v, Ψ (vs ++ [v]) }}) (λ vs, ∃ v, ⌜eval_manyop op vs = Some v⌝ ∗ Φ v) es [] -∗
+    WPaexp (AExp_Manyop op es ann) {{ Φ }}.
+  Proof.
+    rewrite wp_a_exp_unfold.
+    iIntros "Hes" (regs) "Hregs".
+    rewrite -{2}(app_nil_l es).
+    have : Forall2 (λ e v, eval_a_exp regs e = Some v) [] [] by constructor.
+    move: (@nil a_exp) => es'.
+    move: {1 3}(@nil base_val) => vs Hall.
+    iInduction es as [|e es] "IH" forall (es' vs Hall) => /=.
+    - rewrite right_id.
+      iDestruct "Hes" as (v Hv) "HΦ".
+      iExists _. iFrame. iPureIntro. simpl.
+      erewrite mapM_Some_2; [|done]. done.
+    - rewrite wp_a_exp_unfold.
+      iDestruct ("Hes" with "Hregs") as (v Hv) "[Hregs HΦ]".
+      rewrite (cons_middle e) !app_assoc.
+      iApply ("IH" with "[] HΦ Hregs").
+      iPureIntro. apply: Forall2_app; [done|].
+      constructor; [done|]. constructor.
+  Qed.
+
   Lemma wpe_unop op e Φ ann:
     WPexp e {{ v1, ∃ v, ⌜eval_unop op v1 = Some v⌝ ∗ Φ v}} -∗
     WPexp (Unop op e ann) {{ Φ }}.
   Proof.
     rewrite wp_exp_unfold. iDestruct 1 as (? Hv ??) "HΦ".
     rewrite wp_exp_unfold. iExists _ => /=. iFrame. by rewrite Hv /=.
+  Qed.
+
+  Lemma wpae_unop op e Φ ann:
+    WPaexp e {{ v1, ∃ v, ⌜eval_unop op v1 = Some v⌝ ∗ Φ v}} -∗
+    WPaexp (AExp_Unop op e ann) {{ Φ }}.
+  Proof.
+    rewrite !wp_a_exp_unfold. iIntros "Hexp" (?) "Hregs".
+    iDestruct ("Hexp" with "Hregs") as (? Hv) "[Hregs [%v' [% HΦ]]]".
+    iExists _ => /=. iFrame. by rewrite Hv /=.
   Qed.
 
   Lemma wpe_binop op e1 e2 Φ ann:
@@ -678,6 +843,16 @@ Section exp_lifting.
     rewrite wp_exp_unfold. iExists _ => /=. iFrame. by rewrite Hv1 Hv2 /=.
   Qed.
 
+  Lemma wpae_binop op e1 e2 Φ ann:
+    WPaexp e1 {{ v1, WPaexp e2 {{ v2, ∃ v, ⌜eval_binop op v1 v2 = Some v⌝ ∗ Φ v}} }} -∗
+    WPaexp (AExp_Binop op e1 e2 ann) {{ Φ }}.
+  Proof.
+    rewrite !wp_a_exp_unfold. iIntros "Hexp" (?) "Hregs".
+    iDestruct ("Hexp" with "Hregs") as (? Hv1) "[Hregs He2]".
+    rewrite wp_a_exp_unfold. iDestruct ("He2" with "Hregs") as (? Hv2) "[Hregs [%v' [% HΦ]]]".
+    iExists _ => /=. iFrame. by rewrite Hv1 Hv2 /=.
+  Qed.
+
   Lemma wpe_ite e1 e2 e3 Φ ann:
     WPexp e1 {{ v1, WPexp e2 {{ v2, WPexp e3 {{ v3,
        ∃ b, ⌜v1 = Val_Bool b⌝ ∗ Φ (ite b v2 v3)}} }} }} -∗
@@ -687,6 +862,19 @@ Section exp_lifting.
     rewrite wp_exp_unfold. iDestruct "He2" as (? Hv2) "He3".
     rewrite wp_exp_unfold. iDestruct "He3" as (? Hv3 ? Hv) "HΦ".
     rewrite wp_exp_unfold. iExists _ => /=. iFrame. iPureIntro. simplify_eq.
+    rewrite Hv1 Hv2 Hv3. by case_match.
+  Qed.
+
+  Lemma wpae_ite e1 e2 e3 Φ ann:
+    WPaexp e1 {{ v1, WPaexp e2 {{ v2, WPaexp e3 {{ v3,
+       ∃ b, ⌜v1 = Val_Bool b⌝ ∗ Φ (ite b v2 v3)}} }} }} -∗
+    WPaexp (AExp_Ite e1 e2 e3 ann) {{ Φ }}.
+  Proof.
+    rewrite !wp_a_exp_unfold. iIntros "He1" (?) "Hregs".
+    iDestruct ("He1" with "Hregs") as (? Hv1) "[Hregs He2]".
+    rewrite wp_a_exp_unfold. iDestruct ("He2" with "Hregs") as (? Hv2) "[Hregs He3]".
+    rewrite wp_a_exp_unfold. iDestruct ("He3" with "Hregs") as (? Hv3) "[Hregs [%b [% HΦ]]]".
+    iExists _ => /=. iFrame. iPureIntro. simplify_eq.
     rewrite Hv1 Hv2 Hv3. by case_match.
   Qed.
 
