instructions/binary_search/a3c.v
@@ -2,6 +2,9 @@ From isla Require Import isla_lang.
 
 Definition a3c : list trc := [
   [
+    AssumeReg "PSTATE" [Field "EL"] (RegVal_Base (Val_Bits [BV{2%N} 0x2%Z])) Mk_annot;
+    AssumeReg "PSTATE" [Field "nRW"] (RegVal_Base (Val_Bits [BV{1%N} 0x0%Z])) Mk_annot;
+    AssumeReg "SCR_EL3" [] (RegVal_Base (Val_Bits [BV{32%N} 0x0%Z])) Mk_annot;
     Smt (DeclareConst 49%Z (Ty_BitVec 64%N)) Mk_annot;
     ReadReg "R22" [] (RegVal_Base (Val_Symbolic 49%Z)) Mk_annot;
     Smt (DefineConst 50%Z (Val (Val_Symbolic 49%Z) Mk_annot)) Mk_annot;
