instructions/binary_search/a50.v
@@ -18,6 +18,21 @@ Definition a50 : list trc := [
     ReadReg "PSTATE" [Field "Z"] (RegVal_Struct [("Z", RegVal_Base (Val_Symbolic 27%Z))]) Mk_annot;
     Smt (DefineConst 38%Z (Binop (Eq) (Val (Val_Symbolic 27%Z) Mk_annot) (Val (Val_Bits [BV{1%N} 0x0%Z]) Mk_annot) Mk_annot)) Mk_annot;
     Branch 1%Z "model/aarch64.sail 12137:4 - 12139:5" Mk_annot;
+    Smt (Assert (Unop (Not) (Val (Val_Symbolic 38%Z) Mk_annot) Mk_annot)) Mk_annot
+  ];
+  [
+    Smt (DeclareConst 5%Z (Ty_BitVec 1%N)) Mk_annot;
+    Smt (DeclareConst 27%Z (Ty_BitVec 1%N)) Mk_annot;
+    AssumeReg "PSTATE" [Field "EL"] (RegVal_Base (Val_Bits [BV{2%N} 0x2%Z])) Mk_annot;
+    AssumeReg "PSTATE" [Field "nRW"] (RegVal_Base (Val_Bits [BV{1%N} 0x0%Z])) Mk_annot;
+    AssumeReg "SCR_EL3" [] (RegVal_Base (Val_Bits [BV{32%N} 0x0%Z])) Mk_annot;
+    ReadReg "PSTATE" [Field "C"] (RegVal_Struct [("C", RegVal_Base (Val_Symbolic 5%Z))]) Mk_annot;
+    Smt (DefineConst 37%Z (Binop (Eq) (Val (Val_Symbolic 5%Z) Mk_annot) (Val (Val_Bits [BV{1%N} 0x1%Z]) Mk_annot) Mk_annot)) Mk_annot;
+    Branch 0%Z "model/aarch64.sail 11344:19 - 11344:52" Mk_annot;
+    Smt (Assert (Val (Val_Symbolic 37%Z) Mk_annot)) Mk_annot;
+    ReadReg "PSTATE" [Field "Z"] (RegVal_Struct [("Z", RegVal_Base (Val_Symbolic 27%Z))]) Mk_annot;
+    Smt (DefineConst 38%Z (Binop (Eq) (Val (Val_Symbolic 27%Z) Mk_annot) (Val (Val_Bits [BV{1%N} 0x0%Z]) Mk_annot) Mk_annot)) Mk_annot;
+    Branch 1%Z "model/aarch64.sail 12137:4 - 12139:5" Mk_annot;
     Smt (Assert (Val (Val_Symbolic 38%Z) Mk_annot)) Mk_annot;
     Smt (DeclareConst 39%Z (Ty_BitVec 64%N)) Mk_annot;
     ReadReg "_PC" [] (RegVal_Base (Val_Symbolic 39%Z)) Mk_annot;
@@ -35,17 +50,5 @@ Definition a50 : list trc := [
     ReadReg "TCR_EL2" [] (RegVal_Base (Val_Bits [BV{64%N} 0x0%Z])) Mk_annot;
     WriteReg "_PC" [] (RegVal_Base (Val_Symbolic 53%Z)) Mk_annot;
     WriteReg "__PC_changed" [] (RegVal_Base (Val_Bool true)) Mk_annot
-  ];
-  [
-    Smt (DeclareConst 5%Z (Ty_BitVec 1%N)) Mk_annot;
-    Smt (DeclareConst 27%Z (Ty_BitVec 1%N)) Mk_annot;
-    ReadReg "PSTATE" [Field "C"] (RegVal_Struct [("C", RegVal_Base (Val_Symbolic 5%Z))]) Mk_annot;
-    Smt (DefineConst 37%Z (Binop (Eq) (Val (Val_Symbolic 5%Z) Mk_annot) (Val (Val_Bits [BV{1%N} 0x1%Z]) Mk_annot) Mk_annot)) Mk_annot;
-    Branch 0%Z "model/aarch64.sail 11344:19 - 11344:52" Mk_annot;
-    Smt (Assert (Val (Val_Symbolic 37%Z) Mk_annot)) Mk_annot;
-    ReadReg "PSTATE" [Field "Z"] (RegVal_Struct [("Z", RegVal_Base (Val_Symbolic 27%Z))]) Mk_annot;
-    Smt (DefineConst 38%Z (Binop (Eq) (Val (Val_Symbolic 27%Z) Mk_annot) (Val (Val_Bits [BV{1%N} 0x0%Z]) Mk_annot) Mk_annot)) Mk_annot;
-    Branch 1%Z "model/aarch64.sail 12137:4 - 12139:5" Mk_annot;
-    Smt (Assert (Unop (Not) (Val (Val_Symbolic 38%Z) Mk_annot) Mk_annot)) Mk_annot
   ]
 ].
