instructions/binary_search/a78.v
@@ -16,14 +16,6 @@ Definition a78 : list trc := [
   ];
   [
     Smt (DeclareConst 5%Z (Ty_BitVec 1%N)) Mk_annot;
-    ReadReg "PSTATE" [Field "C"] (RegVal_Struct [("C", RegVal_Base (Val_Symbolic 5%Z))]) Mk_annot;
-    Smt (DefineConst 38%Z (Binop (Eq) (Val (Val_Symbolic 5%Z) Mk_annot) (Val (Val_Bits [BV{1%N} 0x1%Z]) Mk_annot) Mk_annot)) Mk_annot;
-    Branch 0%Z "model/aarch64.sail 11344:19 - 11344:52" Mk_annot;
-    Smt (Assert (Unop (Not) (Val (Val_Symbolic 38%Z) Mk_annot) Mk_annot)) Mk_annot;
-    WriteReg "R0" [] (RegVal_Base (Val_Bits [BV{64%N} 0x1%Z])) Mk_annot
-  ];
-  [
-    Smt (DeclareConst 5%Z (Ty_BitVec 1%N)) Mk_annot;
     Smt (DeclareConst 27%Z (Ty_BitVec 1%N)) Mk_annot;
     ReadReg "PSTATE" [Field "C"] (RegVal_Struct [("C", RegVal_Base (Val_Symbolic 5%Z))]) Mk_annot;
     Smt (DefineConst 38%Z (Binop (Eq) (Val (Val_Symbolic 5%Z) Mk_annot) (Val (Val_Bits [BV{1%N} 0x1%Z]) Mk_annot) Mk_annot)) Mk_annot;
@@ -33,6 +25,14 @@ Definition a78 : list trc := [
     Smt (DefineConst 39%Z (Binop (Eq) (Val (Val_Symbolic 27%Z) Mk_annot) (Val (Val_Bits [BV{1%N} 0x0%Z]) Mk_annot) Mk_annot)) Mk_annot;
     Branch 1%Z "model/aarch64.sail 11370:4 - 11380:5" Mk_annot;
     Smt (Assert (Unop (Not) (Val (Val_Symbolic 39%Z) Mk_annot) Mk_annot)) Mk_annot;
+    WriteReg "R0" [] (RegVal_Base (Val_Bits [BV{64%N} 0x1%Z])) Mk_annot
+  ];
+  [
+    Smt (DeclareConst 5%Z (Ty_BitVec 1%N)) Mk_annot;
+    ReadReg "PSTATE" [Field "C"] (RegVal_Struct [("C", RegVal_Base (Val_Symbolic 5%Z))]) Mk_annot;
+    Smt (DefineConst 38%Z (Binop (Eq) (Val (Val_Symbolic 5%Z) Mk_annot) (Val (Val_Bits [BV{1%N} 0x1%Z]) Mk_annot) Mk_annot)) Mk_annot;
+    Branch 0%Z "model/aarch64.sail 11344:19 - 11344:52" Mk_annot;
+    Smt (Assert (Unop (Not) (Val (Val_Symbolic 38%Z) Mk_annot) Mk_annot)) Mk_annot;
     WriteReg "R0" [] (RegVal_Base (Val_Bits [BV{64%N} 0x1%Z])) Mk_annot
   ]
 ].
