instructions/memcpy/a8.v
@@ -2,10 +2,18 @@ From isla Require Import isla_lang.
 
 Definition a8 : list trc := [
   [
+    AssumeReg "EDSCR" [] (RegVal_Base (Val_Bits [BV{32%N} 0x0%Z])) Mk_annot;
+    AssumeReg "OSDLR_EL1" [] (RegVal_Base (Val_Bits [BV{32%N} 0x0%Z])) Mk_annot;
+    AssumeReg "OSLSR_EL1" [] (RegVal_Base (Val_Bits [BV{32%N} 0x0%Z])) Mk_annot;
     Smt (DeclareConst 6%Z (Ty_BitVec 1%N)) Mk_annot;
+    AssumeReg "PSTATE" [Field "EL"] (RegVal_Base (Val_Bits [BV{2%N} 0x2%Z])) Mk_annot;
+    AssumeReg "PSTATE" [Field "nRW"] (RegVal_Base (Val_Bits [BV{1%N} 0x0%Z])) Mk_annot;
+    AssumeReg "SCR_EL3" [] (RegVal_Base (Val_Bits [BV{32%N} 0x0%Z])) Mk_annot;
+    AssumeReg "SCTLR_EL2" [] (RegVal_Base (Val_Bits [BV{64%N} 0x4000002%Z])) Mk_annot;
     Smt (DeclareConst 29%Z (Ty_BitVec 64%N)) Mk_annot;
     Smt (DeclareConst 30%Z (Ty_BitVec 64%N)) Mk_annot;
-    Smt (Assert (Binop (Eq) (Manyop (Bvmanyarith Bvand) [Manyop (Bvmanyarith Bvadd) [Val (Val_Symbolic 29%Z) Mk_annot; Val (Val_Symbolic 30%Z) Mk_annot] Mk_annot; Val (Val_Bits [BV{64%N} 0xfff0000000000007%Z]) Mk_annot] Mk_annot) (Val (Val_Bits [BV{64%N} 0x0%Z]) Mk_annot) Mk_annot)) Mk_annot;
+    Assume (AExp_Binop (Eq) (AExp_Manyop (Bvmanyarith Bvand) [AExp_Manyop (Bvmanyarith Bvadd) [AExp_Val (AVal_Var "R1" []) Mk_annot; AExp_Val (AVal_Var "R3" []) Mk_annot] Mk_annot; AExp_Val (AVal_Bits [BV{64%N} 0xfff0000000000000%Z]) Mk_annot] Mk_annot) (AExp_Val (AVal_Bits [BV{64%N} 0x0%Z]) Mk_annot) Mk_annot) Mk_annot;
+    Smt (Assert (Binop (Eq) (Manyop (Bvmanyarith Bvand) [Manyop (Bvmanyarith Bvadd) [Val (Val_Symbolic 29%Z) Mk_annot; Val (Val_Symbolic 30%Z) Mk_annot] Mk_annot; Val (Val_Bits [BV{64%N} 0xfff0000000000000%Z]) Mk_annot] Mk_annot) (Val (Val_Bits [BV{64%N} 0x0%Z]) Mk_annot) Mk_annot)) Mk_annot;
     ReadReg "R3" [] (RegVal_Base (Val_Symbolic 30%Z)) Mk_annot;
     ReadReg "R1" [] (RegVal_Base (Val_Symbolic 29%Z)) Mk_annot;
     Smt (DefineConst 103%Z (Manyop (Bvmanyarith Bvadd) [Val (Val_Symbolic 29%Z) Mk_annot; Val (Val_Symbolic 30%Z) Mk_annot] Mk_annot)) Mk_annot;
