pkvm_handler/a7404.v
@@ -2,6 +2,11 @@ From isla Require Import isla_lang.
 
 Definition a7404 : list trc := [
   [
+    AssumeReg "PSTATE" [Field "EL"] (RegVal_Base (Val_Bits [BV{2%N} 0x2%Z])) Mk_annot;
+    AssumeReg "PSTATE" [Field "SP"] (RegVal_Base (Val_Bits [BV{1%N} 0x1%Z])) Mk_annot;
+    AssumeReg "SCR_EL3" [] (RegVal_Base (Val_Bits [BV{32%N} 0x0%Z])) Mk_annot;
+    AssumeReg "SCTLR_EL1" [] (RegVal_Base (Val_Bits [BV{64%N} 0x4000002%Z])) Mk_annot;
+    AssumeReg "SCTLR_EL2" [] (RegVal_Base (Val_Bits [BV{64%N} 0x4000002%Z])) Mk_annot;
     ReadReg "PSTATE" [Field "EL"] (RegVal_Struct [("EL", RegVal_Base (Val_Bits [BV{2%N} 0x2%Z]))]) Mk_annot;
     ReadReg "HCR_EL2" [] (RegVal_Base (Val_Bits [BV{64%N} 0x0%Z])) Mk_annot;
     ReadReg "SCTLR_EL1" [] (RegVal_Base (Val_Bits [BV{64%N} 0x4000002%Z])) Mk_annot;
