pkvm_handler/a7418.v
@@ -2,10 +2,6 @@ From isla Require Import isla_lang.
 
 Definition a7418 : list trc := [
   [
-    Smt (DeclareConst 5%Z (Ty_BitVec 1%N)) Mk_annot;
-    Smt (DeclareConst 17%Z (Ty_BitVec 1%N)) Mk_annot;
-    Smt (DeclareConst 26%Z (Ty_BitVec 1%N)) Mk_annot;
-    Smt (DeclareConst 27%Z (Ty_BitVec 1%N)) Mk_annot;
     Smt (DeclareConst 38%Z (Ty_BitVec 64%N)) Mk_annot;
     ReadReg "R0" [] (RegVal_Base (Val_Symbolic 38%Z)) Mk_annot;
     Smt (DefineConst 39%Z (Val (Val_Symbolic 38%Z) Mk_annot)) Mk_annot;
@@ -13,16 +9,12 @@ Definition a7418 : list trc := [
     Smt (DefineConst 48%Z (Unop (Extract 63%N 0%N) (Val (Val_Symbolic 44%Z) Mk_annot) Mk_annot)) Mk_annot;
     Smt (DefineConst 61%Z (Manyop Concat [Manyop Concat [Manyop Concat [Manyop (Bvmanyarith Bvor) [Manyop (Bvmanyarith Bvand) [Val (Val_Bits [BV{1%N} 0x0%Z]) Mk_annot; Unop (Bvnot) (Val (Val_Bits [BV{1%N} 0x1%Z]) Mk_annot) Mk_annot] Mk_annot; Unop (Extract 0%N 0%N) (Binop ((Bvarith Bvlshr)) (Val (Val_Symbolic 48%Z) Mk_annot) (Unop (Extract 63%N 0%N) (Val (Val_Bits [BV{128%N} 0x3f%Z]) Mk_annot) Mk_annot) Mk_annot) Mk_annot] Mk_annot; Ite (Binop (Eq) (Val (Val_Symbolic 48%Z) Mk_annot) (Val (Val_Bits [BV{64%N} 0x0%Z]) Mk_annot) Mk_annot) (Val (Val_Bits [BV{1%N} 0x1%Z]) Mk_annot) (Val (Val_Bits [BV{1%N} 0x0%Z]) Mk_annot) Mk_annot] Mk_annot; Ite (Binop (Eq) (Unop (ZeroExtend 64%N) (Val (Val_Symbolic 48%Z) Mk_annot) Mk_annot) (Val (Val_Symbolic 44%Z) Mk_annot) Mk_annot) (Val (Val_Bits [BV{1%N} 0x0%Z]) Mk_annot) (Val (Val_Bits [BV{1%N} 0x1%Z]) Mk_annot) Mk_annot] Mk_annot; Ite (Binop (Eq) (Unop (SignExtend 64%N) (Val (Val_Symbolic 48%Z) Mk_annot) Mk_annot) (Manyop (Bvmanyarith Bvadd) [Manyop (Bvmanyarith Bvadd) [Unop (SignExtend 64%N) (Val (Val_Symbolic 39%Z) Mk_annot) Mk_annot; Val (Val_Bits [BV{128%N} 0xfffffffffffffffffffffffffffffffc%Z]) Mk_annot] Mk_annot; Val (Val_Bits [BV{128%N} 0x1%Z]) Mk_annot] Mk_annot) Mk_annot) (Val (Val_Bits [BV{1%N} 0x0%Z]) Mk_annot) (Val (Val_Bits [BV{1%N} 0x1%Z]) Mk_annot) Mk_annot] Mk_annot)) Mk_annot;
     Smt (DefineConst 63%Z (Unop (Extract 3%N 3%N) (Val (Val_Symbolic 61%Z) Mk_annot) Mk_annot)) Mk_annot;
-    ReadReg "PSTATE" [Field "N"] (RegVal_Struct [("N", RegVal_Base (Val_Symbolic 17%Z))]) Mk_annot;
     WriteReg "PSTATE" [Field "N"] (RegVal_Struct [("N", RegVal_Base (Val_Symbolic 63%Z))]) Mk_annot;
     Smt (DefineConst 64%Z (Unop (Extract 2%N 2%N) (Val (Val_Symbolic 61%Z) Mk_annot) Mk_annot)) Mk_annot;
-    ReadReg "PSTATE" [Field "Z"] (RegVal_Struct [("Z", RegVal_Base (Val_Symbolic 27%Z))]) Mk_annot;
     WriteReg "PSTATE" [Field "Z"] (RegVal_Struct [("Z", RegVal_Base (Val_Symbolic 64%Z))]) Mk_annot;
     Smt (DefineConst 65%Z (Unop (Extract 1%N 1%N) (Val (Val_Symbolic 61%Z) Mk_annot) Mk_annot)) Mk_annot;
-    ReadReg "PSTATE" [Field "C"] (RegVal_Struct [("C", RegVal_Base (Val_Symbolic 5%Z))]) Mk_annot;
     WriteReg "PSTATE" [Field "C"] (RegVal_Struct [("C", RegVal_Base (Val_Symbolic 65%Z))]) Mk_annot;
     Smt (DefineConst 66%Z (Unop (Extract 0%N 0%N) (Val (Val_Symbolic 61%Z) Mk_annot) Mk_annot)) Mk_annot;
-    ReadReg "PSTATE" [Field "V"] (RegVal_Struct [("V", RegVal_Base (Val_Symbolic 26%Z))]) Mk_annot;
     WriteReg "PSTATE" [Field "V"] (RegVal_Struct [("V", RegVal_Base (Val_Symbolic 66%Z))]) Mk_annot
   ]
 ].
