pkvm_handler/a7420.v
@@ -2,6 +2,8 @@ From isla Require Import isla_lang.
 
 Definition a7420 : list trc := [
   [
+    AssumeReg "PSTATE" [Field "EL"] (RegVal_Base (Val_Bits [BV{2%N} 0x2%Z])) Mk_annot;
+    AssumeReg "PSTATE" [Field "SP"] (RegVal_Base (Val_Bits [BV{1%N} 0x1%Z])) Mk_annot;
     ReadReg "PSTATE" [Field "SP"] (RegVal_Struct [("SP", RegVal_Base (Val_Bits [BV{1%N} 0x1%Z]))]) Mk_annot;
     ReadReg "PSTATE" [Field "EL"] (RegVal_Struct [("EL", RegVal_Base (Val_Bits [BV{2%N} 0x2%Z]))]) Mk_annot;
     Smt (DeclareConst 38%Z (Ty_BitVec 64%N)) Mk_annot;
